Verity/Macro/Syntax.lean
@@ -10,6 +10,7 @@ declare_syntax_cat verityParam
 declare_syntax_cat verityError
 declare_syntax_cat verityConstant
 declare_syntax_cat verityImmutable
+declare_syntax_cat verityExternal
 declare_syntax_cat verityConstructor
 declare_syntax_cat verityFunction
 
@@ -22,6 +23,7 @@ syntax ident " : " term : verityParam
 syntax "error " ident "(" sepBy(term, ",") ")" : verityError
 syntax ident " : " term:max " := " term:max : verityConstant
 syntax ident " : " term:max " := " term:max : verityImmutable
+syntax "external " ident "(" sepBy(term, ",") ")" (" -> " "(" sepBy(term, ",") ")")? : verityExternal
 syntax "revert " ident "(" sepBy(term, ",") ")" : doElem
 syntax "revertError " ident "(" sepBy(term, ",") ")" : doElem
 syntax "requireError " term:max ppSpace ident "(" sepBy(term, ",") ")" : doElem
@@ -37,6 +39,7 @@ syntax (name := verityContractCmd)
   ("errors " verityError+)?
   ("constants " verityConstant+)?
   ("immutables " verityImmutable+)?
+  ("linked_externals " verityExternal+)?
   (verityConstructor)?
   verityFunction+ : command
 
